theories/simulations/msim/WTactics.v
@@ -102,6 +102,14 @@ Ltac state_insert_simpl k1 v1 NODT :=
       |rewrite Heq; clear Heq]
   end.
 
+Ltac simpl_set := repeat
+  match goal with
+  | |- context [?X ∪ ∅] => rewrite (right_id_L ∅ _ X)
+  | |- context [∅ ∪ ?X] => rewrite (left_id_L ∅ _ X)
+  | |- context [?A ∖ ?A] => rewrite (difference_diag_L A)
+  | |- context [?A ∖ ?B ∪ ?B] => idtac "TODO"
+  end.
+
 Ltac _wstep_l :=
   match goal with
   | [ |- environments.envs_entails _ (wsim _ _ _ _ _ _ _ _ _ _ _ (_, tau;; _) _) ] =>
@@ -111,7 +119,16 @@ Ltac _wstep_l :=
   | [ |- environments.envs_entails _ (wsim _ _ _ _ _ _ _ _ _ _ _ (_, trigger (Take _) >>= _) _) ] =>
       let name := fresh "_q" in iApply wsim_take_src; iIntros (name)
   | [ |- environments.envs_entails _ (wsim _ _ _ _ _ _ _ _ _ _ _ (_, trigger (Assume ?P) >>= _) _) ] =>
-      unfold_pre_post_term P; iApply wsim_assume_src; iIntrosFresh "ASM"
+      first [
+        tcsearch constr:(WP P)
+          ltac:(fun c =>
+            iApply (wsim_assume_src_WP _ _ _ _ _ _ _ _ _ _ _ _ _ _ _ (i:=c)); simpl);
+        match goal with
+        | [ |- environments.envs_entails _ (?P' -∗ _)] =>
+          unfold_pre_post_term P'; iIntrosFresh "ASM"; simpl_set
+        end
+      | unfold_pre_post_term P; iApply wsim_assume_src; iIntrosFresh "ASM"
+      ]
   | [ |- environments.envs_entails _ (wsim _ _ _ _ _ _ _ _ _ _ _ (_, trigger (AssumeRes _) >>= _) _) ] =>
       iApply wsim_assume_res_src; iIntrosFresh "ASM"
   | [ |- environments.envs_entails _ (wsim _ _ _ _ _ _ _ _ _ _ _ (_, assume _ >>= _) _) ] =>
@@ -124,10 +141,6 @@ Ltac _wstep_l :=
       let NODS := fresh "NODS" in
       iApply wsim_nodup_src; iIntros (NODS);
       iApply wsim_sget_src; state_lookup_simpl st_src k NODS; clear NODS
-  (* | [ |- environments.envs_entails _ (wsim _ _ _ _ _ _ _ _ _ _ _ (_, unwrapU ?ox >>= _) _) ] =>
-      let name := fresh "_q" in
-      iApply wsim_unwrapU_src; iIntros (name) "%";
-      match goal with [ H: ?x = Some _ |- _ ] => let G := fresh "G" in rename H into G; try rewrite -> G in * end *)
   end.
 Ltac wstep_l_core :=
   _wstep_l; s.
@@ -198,17 +211,18 @@ Ltac _wforce_l :=
   | [ |- environments.envs_entails _ (wsim _ _ _ _ _ _ _ _ _ _ _ (_, trigger (Choose ?T) >>= _) _) ] =>
       iApply wsim_choose_src
   | [ |- environments.envs_entails _ (wsim _ _ _ _ _ _ _ _ _ _ _ (_, trigger (Guarantee ?P) >>= _) _) ] =>
-      unfold_pre_post_term P; iApply wsim_guarantee_src
-      (* first [
+      first [
         tcsearch constr:(WP P)
           ltac:(fun c =>
-          iApply (wsim_guarantee_src_WP _ _ _ _ _ _ _ _ _ _ _ _ _ _ _ (i:=c)); [try set_solver|try set_solver|simpl WP_space]);
+          iApply (wsim_guarantee_src_WP _ _ _ _ _ _ _ _ _ _ _ _ _ _ _ (i:=c));
+          [first [done|set_solver]|first [done|set_solver]|simpl WP_space]
+        );
         match goal with
         | [ |- environments.envs_entails _ (?P' ∗ _)] =>
-          unfold_pre_post_term P'
+          unfold_pre_post_term P'; simpl_set
         end
       | unfold_pre_post_term P; iApply wsim_guarantee_src
-      ] *)
+      ]
   | [ |- environments.envs_entails _ (wsim _ _ _ _ _ _ _ _ _ _ _ (_, unwrapN _ >>= _) _) ] =>
       iApply wsim_unwrapN_src
   | [ |- environments.envs_entails _ (wsim _ _ _ _ _ _ _ _ _ _ _ (_, guarantee _ >>= _) _) ] =>
@@ -232,20 +246,18 @@ Ltac _wforce_r :=
   | [ |- environments.envs_entails _ (wsim _ _ _ _ _ _ _ _ _ _ _ _ (_, trigger (Take _) >>= _)) ] =>
       iApply wsim_take_tgt
   | [ |- environments.envs_entails _ (wsim _ _ _ _ _ _ _ _ _ _ _ _ (_, trigger (Assume ?P) >>= _)) ] =>
-      (* first [
+      first [
         tcsearch constr:(WP P)
           ltac:(fun c =>
-            unshelve iApply (wsim_assume_tgt_WP _ _ _ _ _ _ _ _ _ _ _ _ _ _ _ (i:=c)); s;
-            [first [apply nclose_subseteq|try set_solver]
-            |first [apply nclose_subseteq|try set_solver]
-            |simpl WP_space]
-          );
+          iApply (wsim_assume_tgt_WP _ _ _ _ _ _ _ _ _ _ _ _ _ _ _ (i:=c));
+          [first [done|set_solver]|first [done|set_solver]|simpl WP_space]
+        );
         match goal with
         | [ |- environments.envs_entails _ (?P' ∗ _)] =>
-          unfold_pre_post_term P'
+          unfold_pre_post_term P'; simpl_set
         end
-      | unfold_pre_post_term P; iApply wsim_assume_tgt ] *)
-    unfold_pre_post_term P; iApply wsim_assume_tgt
+      | unfold_pre_post_term P; iApply wsim_assume_tgt
+      ]
   | [ |- environments.envs_entails _ (wsim _ _ _ _ _ _ _ _ _ _ _ _ (_, trigger (AssumeRes _) >>= _)) ] =>
       iApply wsim_assume_res_tgt
   | [ |- environments.envs_entails _ (wsim _ _ _ _ _ _ _ _ _ _ _ _ (_, assume _ >>= _)) ] =>
